[Lean] Added first-class universe level polymorphism

TT-model/syntactics.lean
@@ -14,12 +14,14 @@ infixr:50 " +: " => cons
 
 inductive Term : Type where
   | var : Nat → Term
-  | 𝒰 : Nat → Term
+  | 𝒰 : Term → Term
   | pi : Term → Term → Term
   | abs : Term → Term
   | app : Term → Term → Term
   | mty : Term
   | exf : Term → Term
+  | lvl : Term → Term
+  | lof : Nat → Term
 namespace Term
 
 /-*------------------
@@ -43,24 +45,28 @@ theorem liftComp ξ ζ ς (h : ∀ x, (ξ ∘ ζ) x = ς x) :
 @[simp]
 def rename (ξ : Nat → Nat) : Term → Term
   | var s => var (ξ s)
-  | 𝒰 k => 𝒰 k
-  | pi A B => pi (rename ξ A) (rename (lift ξ) B)
+  | 𝒰 a => 𝒰 (rename ξ a)
+  | pi a b => pi (rename ξ a) (rename (lift ξ) b)
   | abs b => abs (rename (lift ξ) b)
   | app b a => app (rename ξ b) (rename ξ a)
   | mty => mty
   | exf b => exf (rename ξ b)
+  | lvl a => lvl (rename ξ a)
+  | lof k => lof k
 
 -- Renamings compose
 theorem renameComp' ξ ζ ς (h : ∀ x, (ξ ∘ ζ) x = ς x) : ∀ s, (rename ξ ∘ rename ζ) s = rename ς s := by
-  intro s; revert ξ ζ ς h
-  induction s <;> intro ξ ζ ς h <;> simp <;> try constructor
+  intro s; revert ξ ζ ς h; induction s
+  all_goals intro ξ ζ ς h; simp; try constructor
   case var s => rw [← h]; rfl
+  case 𝒰 ih => apply ih; assumption
   case pi.left ih _ => apply ih; assumption
   case pi.right _ ih => apply ih; apply liftComp; assumption
   case abs ih => apply ih; apply liftComp; assumption
   case app ih _ => apply ih; assumption
   case app _ ih => apply ih; assumption
   case exf ih => apply ih; assumption
+  case lvl ih => apply ih; assumption
 
 theorem renameComp ξ ζ s : (rename ξ ∘ rename ζ) s = rename (ξ ∘ ζ) s := by
   apply renameComp'; simp
@@ -112,60 +118,70 @@ theorem upRename ξ σ τ (h : ∀ x, (rename ξ ∘ σ) x = τ x) : ∀ x, (ren
 @[simp]
 def subst (σ : Nat → Term) : Term → Term
   | var s => σ s
-  | 𝒰 k => 𝒰 k
-  | pi A B => pi (subst σ A) (subst (⇑ σ) B)
+  | 𝒰 a => 𝒰 (subst σ a)
+  | pi a b => pi (subst σ a) (subst (⇑ σ) b)
   | abs b => abs (subst (⇑ σ) b)
   | app b a => app (subst σ b) (subst σ a)
   | mty => mty
   | exf b => exf (subst σ b)
+  | lvl a => lvl (subst σ a)
+  | lof k => lof k
 
 -- Substitution extensionality
 theorem substExt σ τ (h : ∀ x, σ x = τ x) : ∀ s, subst σ s = subst τ s := by
-  intro s; revert σ τ h
-  induction s <;> intro σ τ h <;> simp <;> try constructor
+  intro s; revert σ τ h; induction s
+  all_goals intro σ τ h; simp; try constructor
   case var => rw [h]
+  case 𝒰 ih => apply ih; assumption
   case pi.left ih _ => apply ih; assumption
   case pi.right _ ih => apply ih; apply upExt; assumption
   case abs ih => apply ih; apply upExt; assumption
   case app.left ih _ => apply ih; assumption
   case app.right _ ih => apply ih; assumption
   case exf ih => apply ih; assumption
+  case lvl ih => apply ih; assumption
 
 -- Applying var "substitution" does nothing
 theorem substId' σ (h : ∀ x, σ x = var x) : ∀ s, subst σ s = s := by
-  intro s; revert σ h
-  induction s <;> intro σ h <;> simp <;> try constructor
+  intro s; revert σ h; induction s
+  all_goals intro σ h; simp; try constructor
   case var => rw [h]
+  case 𝒰 ih => apply ih; assumption
   case pi.left ih _ => apply ih; assumption
   case pi.right _ ih => apply ih; apply upId; assumption
   case abs ih => apply ih; apply upId; assumption
   case app.left ih _ => apply ih; assumption
   case app.right _ ih => apply ih; assumption
   case exf ih => apply ih; assumption
+  case lvl ih => apply ih; assumption
 
 -- Substitution/renaming compositionality
 theorem substRename' ξ σ τ (h : ∀ x, (σ ∘ ξ) x = τ x) : ∀ s, subst σ (rename ξ s) = subst τ s := by
-  intro s; revert ξ σ τ h
-  induction s <;> intro ξ σ τ h <;> simp <;> try constructor
+  intro s; revert ξ σ τ h; induction s
+  all_goals intro ξ σ τ h; simp; try constructor
   case var => rw [← h]; rfl
+  case 𝒰 ih => apply ih; assumption
   case pi.left ih _ => apply ih; assumption
   case pi.right _ ih => apply ih; apply upLift; assumption
   case abs ih => apply ih; apply upLift; assumption
   case app.left ih _ => apply ih; assumption
   case app.right _ ih => apply ih; assumption
   case exf ih => apply ih; assumption
+  case lvl ih => apply ih; assumption
 
 -- Renaming/substitution compositionality
 theorem renameSubst' ξ σ τ (h : ∀ x, (rename ξ ∘ σ) x = τ x) : ∀ s, rename ξ (subst σ s) = subst τ s := by
-  intro s; revert ξ σ τ h
-  induction s <;> intro ξ σ τ h <;> simp <;> try constructor
+  intro s; revert ξ σ τ h; induction s
+  all_goals intro ξ σ τ h; simp; try constructor
   case var => rw [← h]; rfl
+  case 𝒰 ih => apply ih; assumption
   case pi.left ih _ => apply ih; assumption
   case pi.right _ ih => apply ih; apply upRename; assumption
   case abs ih => apply ih; apply upRename; assumption
   case app.left ih _ => apply ih; assumption
   case app.right _ ih => apply ih; assumption
   case exf ih => apply ih; assumption
+  case lvl ih => apply ih; assumption
 
 -- Lifting commutes with substitution
 theorem upSubst ρ σ τ (h : ∀ x, (subst ρ ∘ σ) x = τ x) : ∀ x, (subst (⇑ ρ) ∘ (⇑ σ)) x = (⇑ τ) x := by
@@ -180,15 +196,17 @@ theorem upSubst ρ σ τ (h : ∀ x, (subst ρ ∘ σ) x = τ x) : ∀ x, (subst
 
 -- Substitution compositionality
 theorem substComp' ρ σ τ (h : ∀ x, (subst ρ ∘ σ) x = τ x) : ∀ s, (subst ρ ∘ subst σ) s = subst τ s := by
-  intro s; revert ρ σ τ h
-  induction s <;> intro ξ σ τ h <;> simp <;> try constructor
+  intro s; revert ρ σ τ h; induction s
+  all_goals intro ξ σ τ h; simp; try constructor
   case var => rw [← h]; rfl
+  case 𝒰 ih => apply ih; assumption
   case pi.left ih _ => apply ih; assumption
   case pi.right _ ih => apply ih; apply upSubst; assumption
   case abs ih => apply ih; apply upSubst; assumption
   case app.left ih _ => apply ih; assumption
   case app.right _ ih => apply ih; assumption
   case exf ih => apply ih; assumption
+  case lvl ih => apply ih; assumption
 
 /-*----------------------------------------------
   Substitution & renaming lemmas, extensionally
@@ -198,6 +216,9 @@ def substId : ∀ s, subst var s = s :=
   substId' var (by simp)
 
 def substRename ξ σ : ∀ s, (subst σ ∘ (rename ξ)) s = subst (σ ∘ ξ) s :=
+  substRename' _ _ (σ ∘ ξ) (by simp)
+
+def substRenamed ξ σ : ∀ s, subst σ (rename ξ s) = subst (σ ∘ ξ) s :=
   substRename' _ _ (σ ∘ ξ) (by simp)
 
 def renameSubst ξ σ : ∀ s, (rename ξ ∘ subst σ) s = subst (rename ξ ∘ σ) s :=
@@ -252,3 +273,9 @@ inductive In : Nat → Term → Ctxt → Prop where
   | here {Γ A} : In 0 (rename succ A) (Γ ∷ A)
   | there {Γ x A B} : In x A Γ → In (succ x) (rename succ A) (Γ ∷ B)
 notation:40 Γ:41 "∋" x:41 "∶" A:41 => In x A Γ
+
+theorem inHere {Γ A A'} (e : A' = rename succ A) : (Γ ∷ A) ∋ 0 ∶ A' := by
+  subst e; apply In.here
+
+theorem inThere {Γ x A A' B} (h : Γ ∋ x ∶ A) (e : A' = rename succ A) : Γ ∷ B ∋ succ x ∶ A' := by
+  subst e; apply In.there; assumption
