TT-model/typing.lean
@@ -1,6 +1,7 @@
 import «TT-model».syntactics
 import «TT-model».reduction
 
+open Nat
 open Term
 
 set_option autoImplicit false
@@ -15,6 +16,10 @@ local infix:40 "≈" => Eqv
 
 inductive Eqv : Term → Term → Prop where
   | β {b a} : app (abs b) a ≈ subst (a +: var) b
+  | 𝒰 {a a'} :
+    a ≈ a' →
+    -----------
+    𝒰 a ≈ 𝒰 a'
   | pi {a a' b b'} :
     a ≈ a' →
     b ≈ b' →
@@ -33,6 +38,10 @@ inductive Eqv : Term → Term → Prop where
     b ≈ b' →
     --------------
     exf b ≈ exf b'
+  | lvl {a a'} :
+    a ≈ a' →
+    -----------
+    lvl a ≈ lvl a'
   | refl {a} : a ≈ a
   | sym {a b} :
     a ≈ b →
@@ -72,10 +81,12 @@ theorem convEqv {a b} : a ⇔ b → a ≈ b
 theorem eqvConv {a b} (r : a ≈ b) : a ⇔ b := by
   induction r
   case β => apply parConv; apply Par.β <;> apply parRefl
+  case 𝒰 => apply conv𝒰; assumption
   case pi => apply convPi <;> assumption
   case abs => apply convAbs; assumption
   case app => apply convApp <;> assumption
   case exf => apply convExf; assumption
+  case lvl => apply convLvl; assumption
   case refl => apply convRefl
   case sym => apply convSym; assumption
   case trans => apply convTrans <;> assumption
@@ -129,13 +140,13 @@ inductive Wtf : (Σ w, idx w) → Prop where
     Γ ⊢ var x ∶ A
   | 𝒰 {Γ j k} :
     ⊢ Γ →
-    j < k →
-    --------------
+    Γ ⊢ j ∶ lvl k →
+    ---------------
     Γ ⊢ 𝒰 j ∶ 𝒰 k
   | pi {Γ A B k} :
     Γ ⊢ A ∶ 𝒰 k →
-    Γ ∷ A ⊢ B ∶ 𝒰 k →
-    ------------------
+    Γ ∷ A ⊢ B ∶ 𝒰 (rename succ k) →
+    --------------------------------
     Γ ⊢ pi A B ∶ 𝒰 k
   | abs {Γ A B b k} :
     Γ ⊢ pi A B ∶ 𝒰 k →
@@ -149,23 +160,48 @@ inductive Wtf : (Σ w, idx w) → Prop where
     Γ ⊢ app b a ∶ subst (a +: var) B
   | mty {Γ k} :
     ⊢ Γ →
-    --------------
-    Γ ⊢ mty ∶ 𝒰 k
+    --------------------
+    Γ ⊢ mty ∶ 𝒰 (lof k)
   | exf {Γ A b k} :
     Γ ⊢ A ∶ 𝒰 k →
     Γ ⊢ b ∶ mty →
     -------------
     Γ ⊢ exf b ∶ A
+  | lvl {Γ a b k} :
+    Γ ⊢ a ∶ lvl b →
+    ----------------------
+    Γ ⊢ lvl a ∶ 𝒰 (lof k)
+  | lof {Γ j k} :
+    j < k →
+    -----------------------
+    Γ ⊢ lof j ∶ lvl (lof k)
+  | trans {Γ i j k} :
+    Γ ⊢ i ∶ lvl j →
+    Γ ⊢ j ∶ lvl k →
+    ---------------
+    Γ ⊢ i ∶ lvl k
   | conv {Γ A B a k} :
     A ≈ B →
     Γ ⊢ a ∶ A →
     Γ ⊢ B ∶ 𝒰 k →
     --------------
     Γ ⊢ a ∶ B
+  | sub {Γ j k A} :
+    Γ ⊢ j ∶ lvl k →
+    Γ ⊢ A ∶ 𝒰 j →
+    ---------------
+    Γ ⊢ A ∶ 𝒰 k
 end
 
 notation:40 "⊢" Γ:40 => Wtf (Sigma.mk wf Γ)
 notation:40 Γ:41 "⊢" a:41 "∶" A:41 => Wtf (Sigma.mk wt (T.mk Γ a A))
+
+theorem wtfApp {Γ A B B' b a}
+  (hpi : Γ ⊢ b ∶ pi A B)
+  (ha : Γ ⊢ a ∶ A)
+  (eB : B' = subst (a +: var) B) :
+  Γ ⊢ app b a ∶ B' := by
+  subst eB; apply Wtf.app <;> assumption
 
 /-*---------------------------------------------
   Lean currently doesn't support induction on
