TT-model/example.lean
@@ -1,0 +1,130 @@
+import «TT-model».typing
+
+open Term
+
+@[simp]
+def idType k := (pi (lvl (lof k)) (pi (𝒰 (var 0)) (pi (var 0) (var 1))))
+
+-- idid : ((j : Level< (lof 4)) → (A : 𝒰 j) → A → A) → ((j : Level< (lof 3)) → (A : 𝒰 j) → A → A)
+-- idid ≔ λ id. id (lof 3) ((j : Level< (lof 3)) → (A : 𝒰 j) → A → A) (λ j. id j)
+-- All of the `sorry`s are boring proofs about context well formedness
+def idid : ⬝ ⊢ (abs (app (app ((app (var 0) (lof 3))) (idType 3)) (abs (app (var 1) (var 0))))) ∶ (pi (idType 4) (idType 3)) := by
+  apply Wtf.abs (k := lof 4)
+  . apply Wtf.pi
+    . apply Wtf.pi
+      . apply Wtf.lvl; apply @Wtf.lof _ 4 5; omega
+      . apply Wtf.pi
+        . apply Wtf.𝒰
+          . sorry
+          . apply Wtf.var
+            . sorry
+            . apply inHere; rfl
+        . apply Wtf.pi
+          . apply Wtf.sub
+            . apply Wtf.var
+              . sorry
+              . apply inThere; apply inHere; rfl; rfl
+            . apply Wtf.var
+              . sorry
+              . apply inHere; rfl
+          . apply Wtf.sub
+            . apply Wtf.var
+              . sorry
+              . apply inThere; apply inThere; apply inHere; rfl; rfl; rfl
+            . apply Wtf.var
+              . sorry
+              . apply inThere; apply inHere; rfl; rfl
+    . apply Wtf.sub
+      . apply @Wtf.lof _ 3; omega
+      . apply Wtf.pi
+        . apply Wtf.lvl; apply @Wtf.lof _ 3 4; omega
+        . apply Wtf.pi
+          . apply Wtf.𝒰
+            . sorry
+            . apply Wtf.var
+              . sorry
+              . apply inHere; rfl
+          . apply Wtf.pi
+            . apply Wtf.sub
+              . apply Wtf.var
+                . sorry
+                . apply inThere; apply inHere; rfl; rfl
+              . apply Wtf.var
+                . sorry
+                . apply inHere; rfl
+            . apply Wtf.sub
+              . apply Wtf.var
+                . sorry
+                . apply inThere; apply inThere; apply inHere; rfl; rfl; rfl
+              . apply Wtf.var
+                . sorry
+                . apply inThere; apply inHere; rfl; rfl
+  . apply wtfApp
+    . apply wtfApp
+      . apply wtfApp
+        . apply Wtf.var
+          . sorry
+          . apply inHere; rfl
+        . apply Wtf.lof; omega
+        . simp; exact ⟨rfl, rfl⟩
+      . apply Wtf.pi
+        . apply Wtf.lvl
+          have lt : 3 < 4 := by omega
+          apply Wtf.lof lt
+        . apply Wtf.pi
+          . apply Wtf.𝒰
+            . sorry
+            . apply Wtf.var
+              . sorry
+              . apply inHere; rfl
+          . apply Wtf.pi
+            . apply Wtf.sub
+              . apply Wtf.var
+                . sorry
+                . apply inThere; apply inHere; rfl; rfl
+              . apply Wtf.var
+                . sorry
+                . apply inHere; rfl
+            . apply Wtf.sub
+              . apply Wtf.var
+                . sorry
+                . apply inThere; apply inThere; apply inHere; rfl; rfl; rfl
+              . apply Wtf.var
+                . sorry
+                . apply inThere; apply inHere; rfl; rfl
+      . simp; exact ⟨rfl, rfl⟩
+    . apply Wtf.abs (k := lof 3)
+      . apply Wtf.pi
+        . apply Wtf.lvl; apply @Wtf.lof _ 3 4; omega
+        . apply Wtf.pi
+          . apply Wtf.𝒰
+            . sorry
+            . apply Wtf.var
+              . sorry
+              . apply inHere; rfl
+          . apply Wtf.pi
+            . apply Wtf.sub
+              . apply Wtf.var
+                . sorry
+                . apply inThere; apply inHere; rfl; rfl
+              . apply Wtf.var
+                . sorry
+                . apply inHere; rfl
+            . apply Wtf.sub
+              . apply Wtf.var
+                . sorry
+                . apply inThere; apply inThere; apply inHere; rfl; rfl; rfl
+              . apply Wtf.var
+                . sorry
+                . apply inThere; apply inHere; rfl; rfl
+      . apply wtfApp
+        . apply Wtf.var
+          . sorry
+          . apply inThere; apply inHere; rfl; rfl
+        . apply Wtf.trans
+          . apply Wtf.var
+            . sorry
+            . apply inHere; rfl
+          . apply Wtf.lof; omega
+        . simp
+    . simp
