TT-model/soundness.lean
@@ -20,7 +20,7 @@ theorem soundness {Γ a A} (h : Γ ⊢ a ∶ A) : Γ ⊨ a ∶ A := by
     match ihA rfl σ hσ with
     | ⟨i, P, h𝒰, hA⟩ =>
     match interps𝒰Inv h𝒰 with
-    | ⟨_, e⟩ =>
+    | ⟨_, ra, _, e⟩ =>
     exists i, P; subst e
     match hA with
     | ⟨PA, hA⟩ =>
@@ -31,12 +31,18 @@ theorem soundness {Γ a A} (h : Γ ⊢ a ∶ A) : Γ ⊨ a ∶ A := by
       match ihB rfl (x +: σ) (semSubstCons hA PAx hσ) with
       | ⟨_, _, h𝒰, hB⟩ =>
       match interps𝒰Inv h𝒰 with
-      | ⟨_, e⟩ => subst e; exact hB
+      | ⟨_, rb, _, e⟩ =>
+      subst e; rw [substRenamed] at rb
+      match confluence ra rb with
+      | ⟨_, ra', rb'⟩ =>
+      rw [parsLofInv ra'] at rb';
+      injection (parsLofInv rb') with e;
+      simp [e, hB]
   case abs ihpi ihb =>
     match ihpi rfl σ hσ with
     | ⟨_, _, h𝒰, hpi⟩ =>
     match interps𝒰Inv h𝒰 with
-    | ⟨_, e⟩ =>
+    | ⟨_, _, _, e⟩ =>
     subst e
     match hpi with
     | ⟨P, hpi⟩ =>
@@ -64,25 +70,91 @@ theorem soundness {Γ a A} (h : Γ ⊢ a ∶ A) : Γ ⊨ a ∶ A := by
     exists i, PB; constructor
     . exact hB
     . apply hb <;> assumption
-  case 𝒰 j lt _ _ =>
-    exists (succ j), (∃ P, ⟦ · ⟧ j ↘ P); constructor
-    . simp; apply interps𝒰; omega
-    . constructor; apply interps𝒰 lt
+  case 𝒰 ih =>
+    match ih rfl σ hσ with
+    | ⟨_, P, hk, hj⟩ =>
+    match interpsLvlInv hk with
+    | ⟨k, rk, e⟩ =>
+    subst e
+    match hj with
+    | ⟨j, rj, lt⟩ =>
+    exists (succ k), (∃ P, ⟦ · ⟧ k ↘ P); constructor
+    . simp; exact interpsBwds (pars𝒰 rk) (interps𝒰 (by omega))
+    . constructor; exact interpsBwds (pars𝒰 rj) (interps𝒰 lt)
   case mty i _ _ =>
-    exists (succ i), (∃ P, ⟦ · ⟧ i ↘ P); constructor
-    . apply interps𝒰; omega
-    . constructor; apply interpsMty
+    refine ⟨succ i, (∃ P, ⟦ · ⟧ i ↘ P), ?_, ?_⟩
+    . exact interps𝒰 (by omega)
+    . constructor; exact interpsMty
   case exf ihb _ _ =>
     match ihb rfl σ hσ with
     | ⟨_, _, hmty, hb⟩ =>
     rw [interpsMtyInv hmty] at hb
     contradiction
+  case lvl k _ iha =>
+    match iha rfl σ hσ with
+    | ⟨_, P, hlvl, ha⟩ =>
+    refine ⟨succ k, (∃ P, ⟦ · ⟧ k ↘ P), ?_, ?_⟩
+    . apply interps𝒰; omega
+    . match interpsLvlInv hlvl with
+      | ⟨_, _, e⟩ =>
+      subst e
+      match ha with
+      | ⟨k, r, _⟩ =>
+      exists (∃ j, · ⇒⋆ lof j ∧ j < k)
+      exact interpsBwds (parsLvl r) interpsLvl
+  case lof j k lt =>
+    refine ⟨0, (∃ j, · ⇒⋆ lof j ∧ j < k), ?_, ?_⟩
+    . exact interpsLvl
+    . exists j, Pars.refl _
+  case trans j k _ ihk _ ihj =>
+    match ihk rfl σ hσ with
+    | ⟨k, Pj, hk, hj⟩ =>
+    match interpsLvlInv hk with
+    | ⟨k, _, ePj⟩ =>
+    subst ePj
+    match hj with
+    | ⟨j, rj, ltjk⟩ =>
+    match ihj rfl σ hσ with
+    | ⟨_, Pi, hj, hi⟩ =>
+    match interpsLvlInv hj with
+    | ⟨j', rj', ePi⟩ =>
+    subst ePi
+    match hi with
+    | ⟨i, r, ltij⟩ =>
+    match confluence rj rj' with
+    | ⟨j'', rj, rj'⟩ =>
+    rw [parsLofInv rj] at rj'
+    injection (parsLofInv rj') with e; subst e
+    refine ⟨_, (∃ j, · ⇒⋆ lof j ∧ j < k), hk, ?_⟩
+    . exists i, r; omega
   case conv iha conv _ _ =>
     match iha rfl σ hσ with
     | ⟨i, P, hA, ha⟩ =>
     exists i, P; constructor
-    . apply interpsConv _ hA; apply convSubst σ; apply eqvConv conv
+    . exact interpsConv (convSubst σ (eqvConv conv)) hA
     . exact ha
+  case sub ihj _ ihA =>
+    match ihA rfl σ hσ with
+    | ⟨_, Pj, h𝒰, hA⟩ =>
+    match interps𝒰Inv h𝒰 with
+    | ⟨j, rj, lt , e⟩ =>
+    subst e
+    match hA with
+    | ⟨P, hA⟩ =>
+    match ihj rfl σ hσ with
+    | ⟨_, Pk, hk, hj⟩ =>
+    match interpsLvlInv hk with
+    | ⟨k, rk, e⟩ =>
+    subst e
+    match hj with
+    | ⟨j', rj', lt'⟩ =>
+    match confluence rj rj' with
+    | ⟨j'', rj, rj'⟩ =>
+    rw [parsLofInv rj'] at rj
+    injection (parsLofInv rj) with e; subst e
+    refine ⟨succ k, (∃ P, ⟦ · ⟧ k ↘ P), ?_, ?_⟩
+    . exact interpsBwds (pars𝒰 rk) (interps𝒰 (by omega))
+    . exists P; exact interpsCumul (by omega) hA
 
 theorem consistency {b} : ¬ ⬝ ⊢ b ∶ mty := by
   intro h; match soundness h var (semSubstNil _) with
